Projet_SAV_ccl.v
@@ -1,6 +1,7 @@
 Add LoadPath "C:\Users\Hp\Documents\Coq\projet_Semantique" as CoqDirectory.
 Add LoadPath "/Users/samuel/Documents/Documents-L3/PolyCours/S2/Sem/projet_Semantique" as CoqDirectory.
 Load Projet_SAV_P5.
+Load Projet_SAV_DecidableEquality.
 
 Theorem krivine_trans_is_stategy :
     forall ks_0 ks_1 : krivineState,
@@ -56,24 +57,23 @@ Proof.
     all : trivial.
 Qed.
 
-Fixpoint concat (s : stack) (p : codeBloc * stack) : stack :=
+Fixpoint concat (s : stack) (c : codeBloc) (e : stack) : stack :=
     match s with
-        |empty_stack => p # empty_stack
-        | p_2 # s_2 => p_2 # concat s_2 p
+        | empty_stack => $ (c, e) # empty_stack
+        | $ (c2, e2) # s_2 => $ (c2, e2) # concat s_2 c e
 end.
 
 Lemma tau_inner_concat :
     forall s0 s1 : stack, forall c1 : codeBloc, forall u : lambdaTermeN,
-        tau_inner (concat s0 (c1, s1)) u = app (tau_inner s0 u) (tau_tuple c1 s1).
+        tau_inner (concat s0 c1 s1) u = app (tau_inner s0 u) (tau_tuple c1 s1).
 Proof.
     intro s; induction s.
     simpl.
     trivial.
 
-    case p; clear p.
     simpl.
-    intro c; intro s0; intro s1; intro c1; intro u.
-    rewrite IHs.
+    intro s0; intro c1; intro u.
+    rewrite IHs2.
     reflexivity.
 Qed.
 
@@ -82,19 +82,19 @@ Lemma not_interacting_with_stack :
     ks_0 km->* ks_1 -> 
     let (p0, s0) := ks_0 in let (p1, s1) := ks_1 in
     let (c0, e0) := p0   in let (c1, e1) := p1   in 
-    forall p : codeBloc * stack, (c0, e0, concat s0 p) km->* (c1, e1, concat s1 p).
+    forall c : codeBloc, forall e: stack, (c0, e0, concat s0 c e) km->* (c1, e1, concat s1 c e).
 Proof.
     apply transitionRelationExt_ind.
     all : intro ks_0; case ks_0; clear ks_0.
     all : intro p; case p; clear p.
     all : intro c0; intro e0; intro s0.
-    intro p; apply refl_km.
+    intro c; intro e; apply refl_km.
     all : intro ks_1; case ks_1; clear ks_1.
     all : intro p; case p; clear p.
     all : intro c1; intro e1; intro s1.
     intro H.
     inversion H.
-    1-4 : intro p0.
+    1-4 : intro c3; intro e3.
     1-4 : apply single_km.
     apply TAccess_O.
     apply TAccess_S.
@@ -104,10 +104,11 @@ Proof.
     intro ks_2; case ks_2; clear ks_2.
     intro p; case p; clear p.
     intro c2; intro e2; intro s2.
-    intro T1; intro P1; intro T2; intro P2; intro p.
-    pose P1' := P1 p.
-    pose P2' := P2 p.
-    apply (concat_km (c0, e0, concat s0 p) (c1, e1, concat s1 p) (c2, e2, concat s2 p)).
+    intro T1; intro P1; intro T2; intro P2.
+    pose P1' := P1 c2 e2.
+    intro c3; intro e3.
+    pose P2' := P2 c2 e2.
+    apply (concat_km (c0, e0, concat s0 c3 e3) (c1, e1, concat s1 c3 e3) (c2, e2, concat s2 c3 e3)).
     all : trivial.
 Qed.
 
@@ -121,7 +122,7 @@ Proof.
     (*induction H.*)
     unfold comp_glob.
     simpl.
-    pose ks_1 := (comp t, (comp u, empty_stack) # empty_stack, empty_stack) : krivineState.
+    pose ks_1 := (comp t, $ (comp u, empty_stack) # empty_stack, empty_stack) : krivineState.
     exists ks_1.
     unfold ks_1.
     simpl.
@@ -141,8 +142,8 @@ Proof.
 
     apply (concat_km
         (Push comp u; (Grab ; comp t), empty_stack, empty_stack)
-        (Grab; comp t, empty_stack, (comp u, empty_stack) # empty_stack)
-        (comp t, (comp u, empty_stack) # empty_stack, empty_stack)).
+        (Grab; comp t, empty_stack, $ (comp u, empty_stack) # empty_stack)
+        (comp t, $ (comp u, empty_stack) # empty_stack, empty_stack)).
     1-2 : apply single_km.
     apply TPush.
     apply TGrab.
@@ -157,7 +158,7 @@ Proof.
     intro Eq.
     rewrite Eq in H0.
     clear Eq x.
-    pose ks_1 := (c, s, concat s0 (comp v, empty_stack)).
+    pose ks_1 := (c, s, concat s0 (comp v) empty_stack).
     exists ks_1.
     unfold ks_1.
     simpl.
@@ -176,8 +177,8 @@ Proof.
 
     apply (concat_km
         (Push comp v; comp t, empty_stack, empty_stack)
-        (comp t, empty_stack, (comp v, empty_stack) # empty_stack)
-        (c, s, concat s0 (comp v, empty_stack))).
+        (comp t, empty_stack, $ (comp v, empty_stack) # empty_stack)
+        (c, s, concat s0 (comp v) empty_stack)).
     apply single_km.
     apply TPush.
 
@@ -189,72 +190,720 @@ Proof.
     trivial.
 Qed.
 
-Lemma propagation_1: forall ks_0 ks_1 : krivineState
-    (ks_0 km-> ks_1) -> tau ks_0 = tau ks_1 \/ tau ks_0 s-> ks_1. 
+Lemma opposed: forall A B : Prop, (A -> B) -> (not B -> not A).
+Proof. auto. Qed.
 
-Lemma propagation_2: forall ks_0 ks_1: krivineState,
-    (ks_0 km->* ks_1) -> 
-        let (p0, s0) := ks_0 in let (c0, e0) := p0 in
-        forall ks_2 : krivineState, comp_glob (tau ks_0) = ks_2 ->
-    exists ks_3, (ks_2 km->* ks_3) /\ tau ks_3 = tau ks_1.
+
+Lemma terminaison_state :
+    forall ks_0 : krivineState, forall t t_1 : lambdaTermeN,
+        state_correctness ks_0 ->
+        t = tau ks_0 ->
+        (t s-> t_1) -> (t <> t_1) ->
+       (* (forall ks_1 : krivineState, ks_0 km->* ks_1 -> t = tau ks_1) -> *)
+        (forall ks_1 ks_2 : krivineState,
+            ks_0 km->* ks_1 -> ks_1 km-> ks_2 ->
+            (tau ks_0 = tau ks_1) ->
+            let (p_1, s_1) := ks_1 in
+            let (c_1, e_1) := p_1 in
+            (forall n : nat, c_1 <> Access n) -> match c_1 with
+                | (Push _; _) => True
+                | (Grab; _) => (t <> tau ks_2)
+                | Access n => True
+                end
+            ).
 Proof.
-    apply transitionRelationExt_ind.
-    all : intro ks_0; case ks_0; clear ks_0.
-    all : intro p; case p; clear p.
-    all : intro c0; intro e0; intro s0.
-    all : intro ks_1; case ks_1; clear ks_1.
-    all : intro p; case p; clear p.
-    all : intro c1; intro e1; intro s1.
-    intro H.
-    rewrite <- H.
-    exists (c1, e1, s1).
-    split.
-    apply refl_km.
-    rewrite comp_and_tau.
-    reflexivity.
+    intro ks_0; intro t; intro t_1; intro SC; intro Eq.
+    rewrite Eq; clear Eq.
+    intro TisPossible; intro TbutNotEq.
+(*    intro H.*)
+    intro ks_1; case ks_1; clear ks_1.
+    intro p; case p; clear p.
+    intro c; intro e; intro s.
+    intro ks_2; case ks_2; clear ks_2.
+    intro p; case p; clear p.
+    intro c2; intro e2; intro s2.
+    case c; clear c.
+    intro Trans.
+    all : auto.
+    intro c.
+    intro H0.
+    intro H1.
+    case_eq s.
+    intro StackEq.
+    rewrite StackEq in H1.
+    inversion H1.
 
-    intro H.
-    all : intro ks_2; case ks_2; clear ks_2.
-    all : intro p; case p; clear p.
-    all : intro c2; intro e2; intro s2.
+    intro c0; intro e0; intro s0.
+    intro EqS.
 
-    unfold comp_glob.
     intro Eq.
-    inversion Eq.
-    rewrite <- H1, <- H2, <- H3 in H.
-    clear Eq H1 H2 H3 c0 e0 s0.
-    inversion H.
-    rewrite <- H5, <- H4, <- H6 in H.
-    rewrite <- H4.
-    clear H5 e1 H4 c1 H6 s1.
-    clear H2 H3 e s.
+    rewrite EqS in H1.
+    inversion H1.
+    rewrite Eq.
+    intro H10; clear H10.
+    rewrite <- H; rewrite <-H in H1; clear H c2.
+    rewrite <- H9; rewrite <-H9 in H1; clear H9 s2.
+    rewrite <- H8 in H1; clear H8 e2.
+    move : TbutNotEq.
+    rewrite Eq.
+    suff : t_1 = tau (c, $ (c0, e0)# e, s0).
+    intro Eq2; rewrite Eq2.
+    trivial.
+    suff : (tau ks_0) s-> (tau (c, $ (c0, e0)# e, s0)).
+    intro H.
+    exact (kv_red_is_functionnal (tau ks_0) t_1 (tau (c, $ (c0, e0)# e, s0)) (conj TisPossible H)).
 
-    exists (c2, e2, s2).
-    split.
-    apply refl_km.
-    rewrite <- (comp_and_tau (tau (c2, e2, s2))).
+    rewrite Eq.
+    unfold tau.
     simpl.
-    rewrite <- H1.
+    apply tau_inner_krivine_sred.
     unfold tau_tuple.
     simpl.
-    reflexivity.
+    suff : state_correctness (Grab ; c, e, s).
+    intro sC2.
+    inversion sC2.
+    destruct H7.
+    suff : List.Forall (fun t => C[ 0 ]( t )) (tau_stack e).
+    2 : apply stack_correctness_is_no_free; assumption.
+    intro ListForall_isCorrect.
+    rewrite (lemma23 (tau_stack e) ListForall_isCorrect).
+    rewrite (lemma16 (tau_code c) 0 (tau_stack e) ListForall_isCorrect ((tau_code c0) [0 <-- tau_stack e0])).
+    simpl.
+    apply (Kevaluation 
+        (tau_code c) [1 <-- tau_stack e]
+        (tau_code c0) [0 <-- tau_stack e0]
+    ).
 
-    unfold comp_glob.
+    pose H7 := krivine_trans_is_stategy ks_0 (Grab ; c, e, s) SC H0.
+    elim H7.
+    trivial.
+Qed.
+
+Lemma grab_is_reachable : forall ks_0 : krivineState, 
+    state_correctness ks_0 ->
+    exists ks_1, ks_0 km->* ks_1 /\ 
+        (let (p0, _) := ks_1 in let (c0, _) := p0 in 
+            match c0 with
+                | Grab; _ => True
+                | _ => False
+            end
+        ).
+Proof.
+    intro ks_0; case ks_0; clear ks_0.
+    intro p; case p; clear p.
+    intro c; intro e.
+    move : c.
+    induction e.
+    intro c.
+    simpl.
+    induction c; intro s.
+    unfold code_correctness.
+    unfold hasAllFreeVarUnder.
+    simpl.
+    lia.
+    intro H.
+    exists (Grab ; c, empty_stack, s).
+    split; trivial.
+    apply refl_km.
+
+    simpl.
+    intro H.
+    destruct H; destruct H0.
+    pose H2 := code_correctness_propagation_push2 c1 c2 empty_stack H.
+    suff : stack_correctness ($ (c1, empty_stack) # s).
+    intro H3.
+    pose H4 := IHc2 ($ (c1, empty_stack) # s) (conj H2 (conj H0 H3)).
+    inversion H4.
+    destruct H5.
+    exists x.
+    split; trivial.
+    apply (concat_km (Push c1; c2, empty_stack, s) (c2, empty_stack, $ (c1, empty_stack) # s) x).
+    apply single_km.
+    apply TPush.
+    trivial.
+    apply top_is_correct; try assumption.
+    apply (code_correctness_propagation_push1 c1 c2 empty_stack H).
+
+    intro c0.
+
+
+    induction c0; intro s; intro sC.
+    induction n.
+    pose ks_2 := (c, e1, s).
+    inversion sC.
+    destruct H0.
+    inversion H0.
+    clear H2 H3 H4 c_0 e_0 tl.
+    assert (state_correctness (c, e1, s)).
+    unfold state_correctness.
+    auto.
+
+    pose ks_1 := IHe1 c s H2.
+    inversion ks_1.
+    exists x.
+    destruct H3.
+    split; trivial.
+    apply (concat_km (Access 0, $ (c, e1) # e2, s) (c, e1, s) x); trivial.
+    apply single_km.
+    apply TAccess_O.
+
+    inversion sC.
+    destruct H0.
+
+
+
+    pose IHe := IHe2 (Access n) s.
+
+    assert (state_correctness (Access n, e2, s)).
+    unfold state_correctness. 
+
+    inversion H0.
+    split; auto.
+    apply (code_correctness_propagation_access n c e1 e2).
+    assumption.
+
+    pose IH := IHe H2.
+    inversion IH.
+    destruct H3.
+    exists x.
+    split; trivial.
+
+    apply (concat_km (Access (S n), $ (c, e1) # e2, s) (Access n, e2, s), x); trivial.
+    apply single_km.
+    apply TAccess_S.
+
+    exists (Grab ; c0, $ (c, e1) # e2, s).
+    split; trivial.
+    apply refl_km.
+
+    pose H3 := IHc0_2 ($ (c0_1, $ (c, e1) # e2) # s).
+    suff : state_correctness (c0_2, $ (c, e1) # e2, $ (c0_1, $ (c, e1) # e2) # s).
+    intro H4.
+    pose H5 := H3 H4.
+    inversion H5.
+    destruct H.
+    exists x.
+    split; trivial.
+    apply (concat_km
+        (Push c0_1; c0_2, $ (c, e1) # e2, s) 
+        (c0_2, $ (c, e1) # e2, $ (c0_1, $ (c, e1) # e2) # s)
+        x); trivial.
+    apply single_km.
+    apply TPush.
+
+    inversion sC.
+    destruct H0.
+    unfold state_correctness.
+    split.
+    2 : split; trivial.
+    Check code_correctness_propagation_push2.
+    apply (code_correctness_propagation_push2 c0_1); trivial.
+
+    inversion H0.
+    apply top_is_correct; trivial.
+    apply (code_correctness_propagation_push1 c0_1 c0_2); trivial.
+Qed.
+
+Lemma propagation_1: forall ks: krivineState,
+    state_correctness ks -> 
+    (forall t_1 : lambdaTermeN, ((tau ks) s->* t_1) -> tau ks = t_1)
+    ->
+    (forall ks_1 : krivineState, (ks km->* ks_1) -> (tau ks = tau ks_1)).
+Proof.
+    intro ks.
+    intro sC.
+    intro H.
+    intro ks_1.
+    intro H0.
+    Check krivine_trans_is_stategy.
+    pose t := krivine_trans_is_stategy ks ks_1 sC H0.
+    destruct t.
+    pose H3 := H (tau ks_1) H1.
+    trivial.
+Qed.
+
+Lemma lemma00 : 
+    forall t : lambdaTermeN,
+    (forall t_1 : lambdaTermeN, t s->* (t_1) -> t = t_1) <->
+    ~ (exists t_1 : lambdaTermeN, t s->* (t_1) /\ t<> t_1).
+Proof.
+    split.
+    intro H.
+    intro H0.
+    inversion H0.
+    destruct H1.
+    pose Abs := H x H1.
+    congruence.
+    intro H1.
+    intro t1.
+    intro H2.
+    suff : not (t <> t1) -> t = t1.
+    intro H3.
+    elim H3; trivial.
+    contradict H1.
+    exists t1.
+    auto.
+
+    pose Cases := decidable_lambda_terme_equality t t1.
+    case Cases.
+    all : move=>//.
+Qed.
+
+Lemma lemma00bis : 
+    forall t : lambdaTermeN,
+    (exists t_1 : lambdaTermeN, t s->* (t_1) /\ t<> t_1)
+    ->
+    not (forall t_1 : lambdaTermeN, t s->* (t_1) -> t = t_1).
+Proof.
+    intro t.
+    intro Exist.
+    inversion Exist.
+    destruct H.
+    intro Forall.
+    pose Eq := Forall x H.
+    congruence.
+Qed.
+
+Lemma lemma01 :
+    forall ks: krivineState,
+        (forall ks_1 : krivineState, ks km->* ks_1 -> tau ks = tau ks_1)
+        <->
+        ~ (exists ks_1 : krivineState, ks km->* ks_1 /\ tau ks <> tau ks_1).
+Proof.
+    split.
+    intro H; intro H0.
+    inversion H0.
+    destruct H1.
+    pose Abs := H x H1.
+    congruence.
+
+    intro NegH.
+    intro ks_1.
+    intro Trans.
+    suff : not (tau ks <> tau ks_1) -> tau ks = tau ks_1.
+    intro H3.
+    elim H3; trivial.
+    contradict NegH.
+    exists ks_1.
+    auto.
+
+    pose Cases := decidable_lambda_terme_equality (tau ks) (tau ks_1).
+    case Cases.
+    all : move => //.
+Qed.
+
+Lemma lemma01bis :
+    forall ks : krivineState,
+        (exists ks_1 : krivineState, ks km->* ks_1 /\ tau ks <> tau ks_1)
+        ->
+        not (forall ks_1 : krivineState, ks km->* ks_1 -> tau ks = tau ks_1).
+Proof.
+    intro ks.
+    intro Exist.
+    intro Forall.
+    inversion Exist.
+    destruct H.
+    pose Abs := Forall x H.
+    congruence.
+Qed.
+
+Lemma propagation_2: forall ks: krivineState,
+    state_correctness ks ->
+    (forall ks_1 : krivineState, (ks km->* ks_1) -> (tau ks = tau ks_1))
+    ->
+    (forall t_1 : lambdaTermeN, ((tau ks) s->* t_1) -> tau ks = t_1).
+Proof.
+    intro ks; intro sC.
+    intro H.
+    assert (~ (exists ks_1 : krivineState, ks km->* ks_1 /\ tau ks <> tau ks_1)).
+    apply (lemma01 ks).
+    assumption.
+
+
+    apply (lemma00 (tau ks)).
+    contradict H0.
+    exfalso.
+
+    inversion H0.
+    destruct H1.
+    induction H1.
+    congruence.
+
+    all : swap 1 2.
+    pose Cases := (decidable_lambda_terme_equality t u).
+    case Cases.
+    intro Eq.
+    rewrite Eq in H1_ H1_0 IHkrivine_red1 IHkrivine_red2 H2 H H0.
+    clear Eq Cases t.
+    apply IHkrivine_red2; trivial.
+    
+    intro NotEq.
+    apply IHkrivine_red1; trivial.
+
+    pose self := refl_km ks.
+    pose Eq := H ks self.
+    assert (forall ks_1 ks_2 : krivineState,
+        ks km->* ks_1 ->
+        (ks_1) km-> (ks_2) ->
+        tau ks = tau ks_1 ->
+        let (p_1, _) := ks_1 in
+        let (c_1, _) := p_1 in
+        (forall n : nat, c_1 <> Access n) ->
+        match c_1 with
+        | Grab ; _ => t <> tau ks_2
+        | _ => True
+    end).
+    exact (terminaison_state ks t u sC Eq H1 H2).
+    rewrite Eq in H1 H0 H2 H3.
+
+    pose H4 := grab_is_reachable ks sC.
+    inversion H4.
+    destruct H5.
+    assert (tau ks = tau x).
+    rewrite <- Eq.
+    exact (H x H5).
+
+    pose next := transitionFunction x.
+    case_eq next.
+
+    all : swap 1 2.
+
+    unfold next.
+    induction x.
+    induction a.
+    case_eq a.
+    1-3 : intro c.
+    3 : intro c0.
+    1,3 : intro eq; rewrite eq in H6; trivial.
+    case_eq b.
+    2 : simpl.
+    2 : discriminate.
+    
+    intro Eq2.
+    rewrite <-Eq in H7.
+    rewrite Eq2 in H7.
+    intro Eq3; rewrite Eq3 in H7.
+    unfold tau in H7.
+    unfold tau_tuple in H7.
+    simpl in H7.
+    rewrite <-Eq in H1.
+
+    pose Abs := only_app_may_be_kv_reduced t u H1.
+    inversion Abs.
+    inversion H8.
+    rewrite H9 in H7.
+    discriminate.
+
+    intro k; intro Transition.
+    suff : ((tau x) s-> (tau k)).
+    intro TransS.
+    unfold next in Transition.
+    apply transitionRelation_is_transitionFunction in Transition.
+    pose transition_ks_0_k := concat_km ks x k H5 (single_km x k Transition).
+    pose Absurdity_Eq := H k transition_ks_0_k.
+    rewrite <-H7 in TransS.
+    rewrite <-Eq in TransS; rewrite <-Eq in H1; rewrite <-Eq in H2.
+    pose LastEq := kv_red_is_functionnal t u (tau k) (conj H1 TransS).
+    rewrite LastEq in H2.
+    rewrite Absurdity_Eq in H2.
+    auto.
+    
+    induction x.
+    induction a.
+    rename a into c; rename b0 into e; rename b into s.
+    case_eq c.
+    1-3: intro c0.
+    3: intro c1.
+    1-3: intro Eq2.
+    1-3: rewrite Eq2 in H6.
+    1, 3: exfalso; trivial.
+
+    case_eq s.
+    intro Eq3; rewrite Eq2 in H7; rewrite Eq3 in H7.
+
+    rewrite <- Eq in H1; rewrite <- Eq in H2; rewrite <-Eq in H7.
+    unfold tau in H7.
+    unfold tau_tuple in H7.
+    simpl in H7.
+    pose Abs := only_app_may_be_kv_reduced t u H1.
+    inversion Abs.
+    inversion H8.
+    rewrite H9 in H7.
+    discriminate.
+
+    intro c1; intro e1; intro s1.
+    intro Eq3.
+    move : Transition.
+    unfold next.
+    rewrite Eq2; rewrite Eq3.
+    simpl.
+    case k.
+    intro p; case p; clear p.
+    intro c2; intro e2; intro s2.
+    intro SomeEq.
+    inversion SomeEq.
+    simpl.
+    apply tau_inner_krivine_sred.
+    unfold tau_tuple.
     simpl.
 
-    intro TH1; intro IH1.
-    intro TH2; intro IH2.
+    suff : (List.Forall isClosed (tau_stack e)).
+    intro LFiC.
+    rewrite (lemma23 (tau_stack e) LFiC).
+    rewrite (lemma16 (tau_code c2) 0 (tau_stack e) LFiC).
+    simpl.
+    apply Kevaluation.
+    apply stack_correctness_is_no_free.
 
-    intro ks_3; case ks_3; clear ks_3.
-    intro p; case p; clear p.
-    intro c3; intro e3; intro s3.
+    suff : (state_correctness (c, e, s)).
+    intro sC3.
+    destruct sC3; destruct H12.
+    trivial.
 
-    intro H; inversion H.
-    rewrite <- H1, <- H2, <- H3 in TH1.
-    rewrite <- H1, <- H2, <- H3 in IH1.
-    clear H H1 H2 H3 c0 e0 s0.
-    pose H0 := IH2 (comp_glob (tau (c1, e1, s1))).
-    assert ((comp (tau (c1, e1, s1)), empty_stack, empty_stack) =
-    (c1, e1, s1)) as H.
-
+    pose sC4 := krivine_trans_is_stategy ks (c, e, s) sC H5.
+    destruct sC4.
+    assumption.
 Qed.
+
+Lemma propagation_3 : forall ks : krivineState,
+    state_correctness ks ->
+    (exists t: lambdaTermeN, ((tau ks) s-> t))
+    ->
+    (exists ks_1 : krivineState, ks km->* ks_1 /\ ((tau ks) s-> (tau ks_1))).
+Proof.
+    intro ks.
+    intro sC.
+    intro H.
+    inversion H.
+    pose Cases := decidable_lambda_terme_equality (tau ks) x.
+    case Cases.
+    intro isEq.
+    exists ks.
+    split.
+    apply refl_km.
+    rewrite isEq; rewrite isEq in H0.
+    assumption.
+
+    intro notEq.
+    suff : (exists t : lambdaTermeN, (tau ks) s->* t /\ (tau ks) <> t).
+    2 : exists x.
+    2 : split; trivial.
+    2 : apply Ksingle; assumption.
+    intro ExistwithNotEq.
+
+    assert (tau ks = tau ks) as Eq. reflexivity.
+
+    pose H2 := lemma00bis (tau ks) ExistwithNotEq.
+    assert (not (forall ks_1 : krivineState, ks km->* ks_1 -> tau ks = tau ks_1)).
+    intro Abs.
+    exact (H2 (propagation_2 ks sC Abs)).
+
+
+    pose H3 := grab_is_reachable ks sC.
+
+    inversion H3.
+    clear Cases.
+    assert (tau ks = tau x0 \/ not (tau ks = tau x0)) as Cases.
+    apply decidable_lambda_terme_equality.
+    case Cases.
+    1-2: clear Cases.
+
+    intro tauKs_is_tau_x0.
+    
+    pose H5 := terminaison_state ks (tau ks) x sC Eq H0 notEq.
+
+    pose next := transitionFunction x0.
+    case_eq next.
+    intro k.
+    unfold next.
+    intro Trans.
+    exists k.
+    apply transitionRelation_is_transitionFunction in Trans.
+    destruct H4.
+    split.
+    apply (concat_km ks x0 k).
+    assumption.
+    exact (single_km _ _ Trans).
+
+    assert (let (p_1, _) := x0 in
+    let (c_1, _) := p_1 in
+    (forall n : nat, c_1 <> Access n) ->
+    match c_1 with
+    | Grab ; _ => tau ks <> tau k
+    | _ => True
+    end) as t.
+    exact (H5 x0 k H4 Trans tauKs_is_tau_x0).
+    clear H5.
+
+    induction x0.
+    rename b into s_x0.
+    induction a.
+    rename a into c_x0; rename b into e_x0.
+    case_eq c_x0.
+    1-3 : intro c.
+    3 : intro c2.
+    1-3: intro Eq_c_x0.
+    1-3 :rewrite Eq_c_x0 in H6.
+    1, 3 : apply False_ind; done.
+
+    rewrite Eq_c_x0 in t.
+    rewrite tauKs_is_tau_x0.
+    assert (state_correctness (c_x0, e_x0, s_x0)).
+    pose stateIsCorrect := krivine_trans_is_stategy ks (c_x0, e_x0, s_x0) sC H4.
+    destruct stateIsCorrect.
+    assumption.
+
+    pose isReduce := trans_is_krivine_reduce (c_x0, e_x0, s_x0) k Trans H5.
+    case isReduce.
+    trivial.
+
+    assert (forall n : nat, Grab; c <> Access n).
+    intro n.
+    discriminate.
+
+    intro AbsEq.
+    pose AbsNEq := t H7.
+    rewrite <- tauKs_is_tau_x0 in AbsEq.
+    congruence.
+
+    unfold next.
+
+    all : swap 1 2.
+
+    intro NotEq.
+
+    inversion H4.
+    pose ind :=  (transitionRelationExt_ind (fun ks x0 =>
+        (tau ks <> tau x0) -> 
+        state_correctness ks ->
+        exists ks_1 : krivineState, ks km->* ks_1 /\ (tau ks) s-> (tau ks_1))).
+    assert (forall ks : krivineState,
+    (fun ks0 x0 : krivineState =>
+     (tau ks <> tau x0) ->
+     state_correctness ks ->
+     exists ks_1 : krivineState,
+       ks0 km->* ks_1 /\ (tau ks0) s-> (tau ks_1))
+      ks ks) as Ind1.
+    intro ks0.
+    congruence.
+
+    assert (forall ks_0 ks_1 : krivineState,
+    (ks_0) km-> (ks_1) ->
+    (fun ks x0 : krivineState =>
+     tau ks <> tau x0 ->
+     state_correctness ks ->
+     exists ks_2 : krivineState,
+       ks km->* ks_2 /\ (tau ks) s-> (tau ks_2))
+      ks_0 ks_1) as Ind2.
+    intro ks_0; intro ks_1.
+    intro Trans.
+    intro NotEq2.
+    intro sC2.
+    pose Cases := trans_is_krivine_reduce ks_0 ks_1 Trans sC2.
+    case Cases; clear Cases.
+    intro Trans2.
+    exists ks_1.
+    split; trivial.
+    apply single_km; assumption.
+    congruence.
+
+
+    assert (forall ks_0 ks_1 ks_2 : krivineState,
+    ks_0 km->* ks_1 ->
+    (fun ks x0 : krivineState =>
+     tau ks <> tau x0 ->
+     state_correctness ks ->
+     exists ks_3 : krivineState,
+       ks km->* ks_3 /\ (tau ks) s-> (tau ks_3))
+      ks_0 ks_1 ->
+    ks_1 km->* ks_2 ->
+    (fun ks x0 : krivineState =>
+     tau ks <> tau x0 ->
+     state_correctness ks ->
+     exists ks_3 : krivineState,
+       ks km->* ks_3 /\ (tau ks) s-> (tau ks_3))
+      ks_1 ks_2 ->
+    (fun ks x0 : krivineState =>
+     tau ks <> tau x0 ->
+     state_correctness ks ->
+     exists ks_3 : krivineState,
+       ks km->* ks_3 /\ (tau ks) s-> (tau ks_3))
+      ks_0 ks_2) as Ind3.
+    intro ks_0; intro ks_1; intro ks_2.
+    intro T1; intro IH1; intro T2; intro IH2; intro NotEq2; intro sC2.
+
+
+    pose Cases := decidable_lambda_terme_equality (tau ks_0) (tau ks_1).
+    case Cases; clear Cases.
+    intro Eq2.
+    rewrite <-Eq2 in IH2.
+    pose sC3 := krivine_trans_is_stategy ks_0 ks_1 sC2 T1.
+    destruct sC3.
+    pose IH := IH2 NotEq2 H8.
+    inversion IH.
+    destruct H9.
+    exists x1.
+    split; trivial.
+    apply (concat_km ks_0 ks_1 x1); assumption.
+
+    intro NotEq3.
+    exact (IH1 NotEq3 sC2).
+
+    pose ind2 := ind Ind1 Ind2 Ind3 ks x0 H5.
+    simpl in ind2.
+    exact (ind2 NotEq sC).
+
+    suff : (forall ks_1 : krivineState, ks km->* ks_1 -> tau ks = tau ks_1).
+    congruence.
+
+    intro ks_1.
+    intro T.
+Admitted.
+
+Lemma propagation_4 : forall t0 t1: lambdaTermeN, t0 s->* t1 ->
+    forall ks : krivineState,  state_correctness ks -> (tau ks) = t0 -> (exists ks_1 : krivineState, ks km->* ks_1 /\ tau ks_1 = t1).
+Proof.
+    intro t0; intro t1.
+    intro T.
+    induction T.
+    all : intro ks; intro sC; intro Eq.
+    exists ks.
+    split.
+    apply refl_km.
+    trivial.
+    
+    pose Cases := decidable_lambda_terme_equality t u.
+    case Cases; clear Cases.
+    intro isEq2.
+    exists ks.
+    rewrite Eq isEq2.
+    split; trivial.
+    apply refl_km.
+
+    intro notEq.
+    rewrite <-Eq in H.
+    assert (exists t : lambdaTermeN, (tau ks) s-> (t)) as ExistT.
+    exists u; assumption.
+    pose ExistK :=  propagation_3 ks sC ExistT.
+    inversion ExistK.
+    destruct H0.
+    exists x.
+    split; trivial.
+    apply (kv_red_is_functionnal (tau ks)).
+    auto.
+
+    pose Exist1 := IHT1 ks sC Eq.
+    inversion Exist1.
+    destruct H.
+
+    pose Trans := krivine_trans_is_stategy ks x sC H.
+    destruct Trans.
+    
+    pose Exist2 := IHT2 x H2 H0.
+    inversion Exist2.
+    destruct H3.
+    exists x0.
+    split; trivial.
+    apply (concat_km ks x x0); assumption.
+Qed.
+
